Add simplified Stack datatype and attached functions. See #486

src/dafny/core/stack.dfy
@@ -19,29 +19,104 @@ module Stack {
     // Maximum stack capcity is 1024 words.
     const CAPACITY : int := 1024;
 
+    type ValidStackContent = xs: seq<u256> | |xs| <= CAPACITY
+
+    datatype Stack = Stack(contents: ValidStackContent) 
+    {
+        // Get number of items currently on this Stack.
+        function method Size(): nat { |contents| }
+
+        // Get remaining capacity of stack (i.e. number of items we could still
+        // push).
+        function method Capacity(): nat {
+            CAPACITY - |contents|
+        }
+
+        // Push word onto Stack.  This requires that there is sufficient space for
+        // that item.
+        function method Push(val: u256): Stack
+            // Sanity check enough space.
+            requires this.Size() < CAPACITY {
+                Stack(contents:=([val] + contents))
+        }
+
+        // Peek nth word from top of Stack (where 0 is top item, 1 is next item, and
+        // so on).  This requires there are sufficiently many words.
+        function method Peek(k: nat) : u256
+            // Sanity check enough items to pop!
+            requires k >= 0 && k < this.Size() {
+                contents[k]
+        }
+
+        // Peek top N words on the Stack.  This requires there are sufficiently many
+        // words.
+        function method PeekN(n: nat) : (r:seq<u256>)
+        requires this.Size() >= n
+        ensures |r| == n {
+                contents[..n]
+        }
+
+        // Pop word off of this Stack.  This requires something to pop!
+        function method Pop(): Stack
+            // Sanity check something to pop.
+            requires this.Size() > 0 {
+                Stack(contents:= contents[1..])
+        }
+
+        // Pop N words off of this Stack.  This requires something to pop!
+        function method PopN(n: nat): Stack
+            // Sanity check something to pop.
+            requires this.Size() >= n {
+                Stack(contents:= contents[n..])
+        }
+
+        /** Swap top item at index 0 and the k+1-th item at index k. */
+        function method Swap(k: nat) : Stack
+        requires this.Size() > k > 0
+        {
+            var top := contents[0];
+            var kth := contents[k];
+            Stack(contents := contents[0:=kth][k:=top])
+        }
+
+        /**
+         *  A sliced stack.
+         *  @param  l   An index.
+         *  @param  u   An index.
+         *  @returns    The stack made of the first u elements minus the first l.
+         */
+        function Slice(l: nat, u: nat): (r: Stack)
+            requires l <= u <= this.Size()
+        {
+            Stack(contents[l..u])
+        }
+
+    }
+
     // A raw stack consistents of a sequence of data, and a stack pointer.
-    datatype Raw = Stack(contents:seq<u256>)
+    // datatype Raw = Stack(contents:seq<u256>)
 
     // A valid Stack cannot exceed the capacity.
-    type T = s:Raw | |s.contents| <= CAPACITY
-    witness Stack([])
+    // type T = s:Raw | |s.contents| <= CAPACITY
+    // witness Stack([])
+    // type T = Stack 
 
-    const Empty := Stack([])
+    const Empty := Stack(contents := [])
 
     // Get number of items currently on this Stack.
-    function method Size(st:T) : nat { |st.contents| }
+    function method Size(st: Stack) : nat { |st.contents| }
 
     // Get remaining capacity of stack (i.e. number of items we could still
     // push).
-    function method Capacity(st:T) : nat {
+    function method Capacity(st: Stack) : nat {
       CAPACITY - |st.contents|
     }
 
     // Create an empty stack.
-    function method Create() : T { Stack(contents:=[]) }
+    function method Create() : Stack { Stack(contents:=[]) }
 
     /** Make a stack with some initial contents.  */
-    function method Make(s: seq<u256>) : T
+    function method Make(s: seq<u256>) : Stack 
         requires |s| <= CAPACITY
     {
         Stack(contents:=s)
@@ -49,7 +124,7 @@ module Stack {
 
     // Push word onto Stack.  This requires that there is sufficient space for
     // that item.
-    function method Push(st:T, val:u256) : T
+    function method Push(st: Stack, val:u256) : Stack 
         // Sanity check enough space.
         requires Size(st) < CAPACITY {
             Stack(contents:=([val] + st.contents))
@@ -57,7 +132,7 @@ module Stack {
 
     // Peek nth word from top of Stack (where 0 is top item, 1 is next item, and
     // so on).  This requires there are sufficiently many words.
-    function method Peek(st:T, k:int) : u256
+    function method Peek(st: Stack, k:int) : u256
         // Sanity check enough items to pop!
         requires k >= 0 && k < Size(st) {
             st.contents[k]
@@ -65,28 +140,28 @@ module Stack {
 
     // Peek top N words on the Stack.  This requires there are sufficiently many
     // words.
-    function method PeekN(st:T, n:nat) : (r:seq<u256>)
+    function method PeekN(st: Stack, n:nat) : (r:seq<u256>)
     requires Size(st) >= n
     ensures |r| == n {
             st.contents[0..n]
     }
 
     // Pop word off of this Stack.  This requires something to pop!
-    function method Pop(st:T) : T
+    function method Pop(st: Stack) : Stack 
         // Sanity check something to pop.
         requires Size(st) > 0 {
             Stack(contents:=st.contents[1..])
     }
 
     // Pop N words off of this Stack.  This requires something to pop!
-    function method PopN(st:T, n:nat) : T
+    function method PopN(st: Stack, n:nat) : Stack 
         // Sanity check something to pop.
         requires Size(st) >= n {
             Stack(contents:=st.contents[n..])
     }
 
     /** Swap top item at index 0 and the k+1-th item at index k. */
-    function method Swap(st:T, k:nat) : T
+    function method Swap(st: Stack, k:nat) : Stack 
       requires Size(st) > k > 0
     {
         var top := st.contents[0];
@@ -101,7 +176,7 @@ module Stack {
      *  @param  u   An index.
      *  @returns    The stack made of the first u elements minus the first l.
      */
-    function Slice(st: T, l: nat, u: nat): (r:T)
+    function Slice(st: Stack, l: nat, u: nat): (r: Stack)
         requires l <= u <= Size(st)
     {
         Stack(st.contents[l..u])
